\documentclass[12pt, a4paper]{article}

\usepackage{blindtext}
\usepackage{geometry}
\geometry{
  a4paper,
  total={170mm,257mm},
  left=20mm,
  top=20mm,
}
\usepackage{amsmath}
\usepackage{amssymb}
\setlength{\parindent}{0pt}

\begin{document}
\section{Question 1}
\begin{itemize}
  \item First Order, Linear, Non-Homogenous
  \item First Order, Linear, Homogenous
  \item Third Order, Non-Linear, Non-Homogenous
  \item Fourth Order, Non-Linear, Non-Homogenous
\end{itemize}

\section{Question 2}
\subsection{(i)}
\begin{gather*}
  \cos^2 t \cdot \frac{d \theta }{ dt } + \cos^2 \theta = 0 \implies
  \frac{d \theta}{\cos^2 \theta} = -\frac{dt}{\cos^2 t} \\[5pt]
  \int \frac{d \theta}{\cos^2 \theta} = -\int \frac{dt}{\cos^2 t} \implies 
  \tan \theta = -\tan t + C \\[5pt]
  \text{When t = } \frac{\pi}{4}, \; \theta = \frac{\pi}{4} \implies C = 2
\end{gather*}

\subsection{(ii)}
\begin{gather*}
  \frac{dy}{dx} + 2x(y + 1) = 0 \implies
  \frac{dy}{y + 1} = -2x \cdot dx \\[5pt]
  \int \frac{dy}{y + 1} = -2 \int x \cdot dx \implies
  \ln |y + 1| = -x^2 + C \\[5pt]
  y + 1 = e^{-Cx^2} 
\end{gather*}
\end{document}
